update COQ files

coq/Example.v
@@ -5,35 +5,26 @@ Require Import String.
 
 Definition es := Apply (Delta (Add_operation (Sym "T" "__libc_start_main@@GLIBC_2.0") (Delta nil)::Add_operation (Sym "T" "__stack_chk_fail@@GLIBC_2.4") (Delta nil)::nil), List ((Sym "T" "__libc_start_main@@GLIBC_2.0")::(Sym "T" "__stack_chk_fail@@GLIBC_2.4")::nil)).
 
-Definition tx := TypedExpression (Delta (Add_operation (Sym "T" "__libc_start_main@@GLIBC_2.0") (Delta nil)::Add_operation (Sym "T" "__stack_chk_fail@@GLIBC_2.4") (Delta nil)::nil),Type_Delta ("T"::"T"::nil)).
+Definition tx := TypedExpression 
+                   (Delta (Add_operation (Sym "T" "__libc_start_main@@GLIBC_2.0") (Delta nil)::
+                           Add_operation (Sym "T" "__stack_chk_fail@@GLIBC_2.4") (Delta nil)::nil),
+                    Type_Delta (("T"::nil) ++ ("T"::nil) ++ nil)).
 
 Definition ty := SafeTable (List ((Sym "T" "__libc_start_main@@GLIBC_2.0")::(Sym "T" "__stack_chk_fail@@GLIBC_2.4")::nil),Type_Delta ("T"::"T"::nil)).
 
-Ltac solve_apply :=
-  repeat match goal with
-          | [ |- Apply (_,_)] => try (replace ((Sym "t" "adsds")::nil) 
-                                      with (((Sym "t" "adsds")::nil) ++ nil) 
-                                       by (rewrite app_nil_r; reflexivity));
-                                repeat (apply APPLY_delta || apply ADD_object || apply EMPTY)
-         end.
-
-Ltac solve_tc :=
-  repeat match goal with
-          | [ |- TypedExpression (_,_)] => try (replace (("t")::nil) 
-                                                with ((("t")::nil) ++ nil) 
-                                                 by (rewrite app_nil_r; reflexivity));
-                                          repeat (apply TE_Delta || apply TE_Symbols_Add || 
-                                                  apply TE_Empty || apply TE_Symbol)
-         end.
-
 Lemma delta: 
-  SafeTable (List ((Sym "t" "adsds")::nil), Type_Delta ("t"::nil)). 
+  SafeTable (List ((Sym "t" "adsds")::nil ++ nil), Type_Delta ("t"::nil)). 
 Proof. 
-  assert (Apply  (Delta ((Add_operation (Sym "t" "adsds") (Delta nil))::nil), List ((Sym "t" "adsds")::nil)))
+
+  assert tx. unfold tx. solve_typed_expr. 
+
+  assert (Apply  (Delta ((Add_operation (Sym "t" "adsds") (Delta nil))::nil), 
+                  List (((Sym "t" "adsds")::nil) ++ nil)))
     by solve_apply.
 
-  assert (TypedExpression (Delta ((Add_operation (Sym "t" "adsds") (Delta nil))::nil), Type_Delta (("t")::nil)))
-    by solve_tc.
+  assert (TypedExpression (Delta ((Add_operation (Sym "t" "adsds") (Delta nil))::nil), 
+                           Type_Delta (("t"::nil) ++ nil )))
+    by solve_typed_expr.
 
   assert (Resolved ("t"::nil))
     by solve_consistency.
